architecture_spec.v
@@ -1,0 +1,128 @@
+(* Copyright (c) 2012-2014, Robbert Krebbers. *)
+(* This file is distributed under the terms of the BSD license. *)
+Require Export type_system.
+Require Import natural_type_environment.
+
+Record architecture := Architecture {
+  big_endian : bool;
+  char_bits_minus8 : nat;
+  char_signedness : signedness;
+  short_bytes_log2 : nat;
+  int_bytes_log2 : nat;
+  long_bytes_log2 : nat → nat;
+  ptr_bytes_log2 : nat;
+  align_minus : nat → nat
+}.
+
+Inductive irank (A : architecture) : Set := IKind { ibytes_log2 : nat }.
+Arguments ibytes_log2 {_} _.
+Instance irank_eq_dec {A} (k1 k2 : irank A) : Decision (k1 = k2).
+Proof. solve_decision. Defined.
+
+Section architecture.
+Context (A : architecture).
+
+Instance: IntCoding (irank A) := {
+  char_rank := IKind A 0;
+  char_signedness := char_signedness A;
+  short_rank := IKind A (short_bytes_log2 A);
+  int_rank := IKind A (int_bytes_log2 A);
+  long_rank n := IKind A (long_bytes_log2 A n);
+  ptr_rank := IKind A (ptr_bytes_log2 A);
+  char_bits := char_bits_minus8 A + 8;
+  rank_size := λ k, 2 ^ ibytes_log2 k;
+  endianize := λ _, if big_endian A then reverse else id;
+  deendianize := λ _, if big_endian A then reverse else id
+}.
+Instance: IntEnv (irank A) := {
+  int_arithop_ok op x τ1 y τ2 :=
+    let τ' := int_promote τ1 ∪ int_promote τ2 in
+    int_pre_arithop_ok op (int_pre_cast τ' x) (int_pre_cast τ' y) τ';
+  int_arithop op x τ1 y τ2 :=
+    let τ' := int_promote τ1 ∪ int_promote τ2 in
+    int_pre_arithop op (int_pre_cast τ' x) (int_pre_cast τ' y) τ';
+  int_shiftop_ok op x τ1 y τ2 :=
+    let τ' := int_promote τ1 in int_pre_shiftop_ok op (int_pre_cast τ' x) y τ';
+  int_shiftop op x τ1 y τ2 :=
+    let τ' := int_promote τ1 in int_pre_shiftop op (int_pre_cast τ' x) y τ';
+  int_cast_ok := int_pre_cast_ok;
+  int_cast := int_pre_cast
+}.
+Instance: IntCodingSpec (irank A).
+Proof.
+  split.
+  * unfold char_bits; simpl; lia.
+  * done.
+  * unfold rank_size; simpl. intros. by apply Nat.neq_0_lt_0, Nat.pow_nonzero.
+  * unfold rank_size; intros [i] [j] ?; simplify_equality'; f_equal.
+    apply Nat.pow_inj_r with 2; lia.
+  * intros. unfold endianize; simpl.
+    by destruct (big_endian _); simpl; rewrite ?reverse_Permutation.
+  * intros. unfold deendianize, endianize; simpl.
+    by destruct (big_endian _); simpl; rewrite ?reverse_involutive.
+  * intros. unfold deendianize, endianize; simpl.
+    by destruct (big_endian _); simpl; rewrite ?reverse_involutive.
+Qed.
+Instance: IntEnvSpec (irank A).
+Proof.
+  split.
+  * apply _.
+  * done.
+  * intros. apply int_pre_arithop_typed; auto.
+    + apply int_pre_cast_typed; auto.
+      by apply int_union_pre_cast_ok_l, int_promote_typed.
+    + apply int_pre_cast_typed; auto.
+      by apply int_union_pre_cast_ok_r, int_promote_typed.
+  * done.
+  * done.
+  * intros. eapply int_pre_shiftop_typed; eauto.
+    apply int_pre_cast_typed; auto.
+    by apply int_typed_pre_cast_ok, int_promote_typed.
+  * unfold int_shiftop; simpl; intros.
+    by rewrite int_typed_pre_cast by auto using int_promote_typed.
+  * done.
+  * intros. by apply int_pre_cast_typed.
+  * done.
+Qed.
+
+Let ptr_size (_ : type (irank A)) : nat := 2 ^ ptr_bytes_log2 A.
+Let align_base (τb : base_type (irank A)) : nat :=
+  match τb with
+  | voidT => 1
+  | intT τi => let n := ibytes_log2 (rank τi) in 2 ^ (n - align_minus A n)
+  | τ.* => let n := ptr_bytes_log2 A in 2 ^ (n - align_minus A n)
+  end%BT.
+Definition align_of : env (irank A) → type (irank A) → nat :=
+  natural_align_of align_base.
+Global Instance architecture_env : Env (irank A) :=
+  natural_env ptr_size align_base.
+
+Let ptr_size_ne_0 τ : ptr_size τ ≠ 0.
+Proof. by apply Nat.pow_nonzero. Qed.
+Let align_void : align_base voidT = 1.
+Proof. done. Qed.
+Let align_int_divide τi : (align_base (intT τi) | rank_size (rank τi)).
+Proof.
+  unfold rank_size; simpl. set (n:=ibytes_log2 (rank τi)).
+  destruct (decide (align_minus A n ≤ n)).
+  { rewrite <-(Nat.sub_add (align_minus A n) n) at 3 by done.
+    rewrite Nat.pow_add_r. by apply Nat.divide_factor_l. }
+  rewrite not_le_minus_0 by done; apply Nat.divide_1_l.
+Qed.
+Let align_ptr_divide τ : (align_base (τ.*) | ptr_size τ).
+Proof.
+  unfold ptr_size; simpl. set (n:=ptr_bytes_log2 A).
+  destruct (decide (align_minus A n ≤ n)).
+  { rewrite <-(Nat.sub_add (align_minus A n) n) at 3 by done.
+    rewrite Nat.pow_add_r. by apply Nat.divide_factor_l. }
+  rewrite not_le_minus_0 by done; apply Nat.divide_1_l.
+Qed.
+
+Global Instance: EnvSpec (irank A).
+Proof. by apply natural_env_spec. Qed.
+Lemma align_of_divide Γ τ : ✓ Γ → ✓{Γ} τ → (align_of Γ τ | size_of Γ τ).
+Proof. by apply natural_align_of_divide. Qed.
+Lemma architecture_field_offset Γ τs i τ :
+  ✓ Γ → ✓{Γ}* τs → τs !! i = Some τ → (align_of Γ τ | field_offset Γ τs i).
+Proof. by apply natural_field_offset. Qed.
+End architecture.
