architectures.v
@@ -1,0 +1,25 @@
+(* Copyright (c) 2012-2014, Robbert Krebbers. *)
+(* This file is distributed under the terms of the BSD license. *)
+Require Export architecture_spec.
+
+Definition x86 := {|
+  big_endian := false;
+  char_bits_minus8 := 0;
+  char_signedness := Signed;
+  short_bytes_log2 := 1;
+  int_bytes_log2 := 2;
+  long_bytes_log2 n := 2 + n;
+  ptr_bytes_log2 := 2;
+  align_minus n := n - 2
+|}.
+
+Definition x86_64 := {|
+  big_endian := false;
+  char_bits_minus8 := 0;
+  char_signedness := Signed;
+  short_bytes_log2 := 1;
+  int_bytes_log2 := 2;
+  long_bytes_log2 n := 2 + n;
+  ptr_bytes_log2 := 3;
+  align_minus n := n - 3
+|}.
