extraction.v
@@ -1,7 +1,7 @@
 (* Copyright (c) 2012-2014, Robbert Krebbers. *)
 (* This file is distributed under the terms of the BSD license. *)
-Require Import interpreter ExtrOcamlBasic ExtrOcamlString.
+Require Import interpreter ExtrOcamlBasic ExtrOcamlString architectures.
 
 Extraction Blacklist list.
 Extraction "parser/Extracted.ml"
-  interpreter.interpreter_all interpreter.interpreter_rand.
+  interpreter.interpreter_all interpreter.interpreter_rand x86.
