natural_type_environment.v
@@ -1,6 +1,6 @@
 (* Copyright (c) 2012-2014, Robbert Krebbers. *)
 (* This file is distributed under the terms of the BSD license. *)
-Require Import type_environment.
+Require Export type_environment.
 
 Section natural_type_environment.
 Context `{IntEnvSpec Ti}.
